ifc-machine/pico/tmu/cmach/Determinism.v
@@ -9,14 +9,13 @@ Require Import Utils.
 Require Import TMUInstr.
 Require Import Abstract Rules AbstractMachine.
 
-Require Import Concrete ConcreteMachine.
+Require Import Concrete ConcreteMachineSmallStep.
 
 Set Implicit Arguments.
 Local Open Scope Z_scope. 
 (* Coercion Z_of_nat : nat >-> Z. *)
 
 Section Determinism.
-
 
 Ltac allinv' :=
   allinv ; 
@@ -25,25 +24,104 @@ Ltac allinv' :=
            H2:  ?f _ _ = _ |- _ ] => rewrite H1 in H2 ; inv H2
      end).
 
+Lemma cache_hit_read_determ: forall c rl1 rpcl1 rl2 rpcl2,
+  cache_hit_read c rl1 rpcl1 -> 
+  cache_hit_read c rl2 rpcl2 ->
+  rl1 = rl2 /\ rpcl1 = rpcl2. 
+Proof.
+  intros. inv H. inv TAG_Res. inv TAG_ResPC. 
+  inv H0. inv TAG_Res. inv TAG_ResPC. 
+  allinv'. allinv'. intuition.
+Qed.
 
 Lemma cmach_priv_determ: 
   forall s s' s'', 
-    cstep_p s s' -> 
-    cstep_p s s'' -> 
+    cstep s s' -> 
+    cstep s s'' -> 
     s' = s''.
 Proof.
-  induction 1; intros; 
+  induction 1; intros;
   match goal with 
-      | [HH: cstep_p _ _ |- _ ] => inv HH; try congruence; auto
+      | [HH: cstep _ _ |- _ ] => inv HH; try congruence; auto
   end;
+  try (match goal with 
+    | [H1 : cache_hit_read ?c ?rl _, 
+       H2 : cache_hit_read ?c ?rl0 _ |- _ ] =>
+  (exploit (@cache_hit_read_determ c rl); eauto; intros [Heq Heq'])
+  end);
   (allinv'; try reflexivity).
   
-  Case "Call".
+  Case "Call user".
     exploit app_same_length_eq; eauto. intro Heq ; inv Heq.
     exploit app_same_length_eq_rest ; eauto. intro Heq ; inv Heq.
     reflexivity.
 
-  Case "Ret".
+  Case "Call kernel".
+    exploit app_same_length_eq; eauto. intro Heq ; inv Heq.
+    exploit app_same_length_eq_rest ; eauto. intro Heq ; inv Heq.
+    reflexivity.
+
+  Case "Ret user".
+    exploit @c_pop_to_return_spec; eauto.
+    intros [dstk [stk [a [b [p [Hs Hdstk]]]]]]. inv Hs.
+    
+    exploit @c_pop_to_return_spec2; eauto.  move_to_top POP0.
+    exploit @c_pop_to_return_spec2; eauto. intros. 
+    inv H. inv H0. 
+    
+    exploit @c_pop_to_return_spec3; eauto. clear POP.
+    exploit @c_pop_to_return_spec3; eauto. 
+    intros.  inv H.    
+    reflexivity.
+
+  Case "Ret kernel / user".
+    exploit @c_pop_to_return_spec; eauto.
+    intros [dstk [stk [a [b [p [Hs Hdstk]]]]]]. inv Hs.
+    
+    exploit @c_pop_to_return_spec2; eauto.  move_to_top POP0.
+    exploit @c_pop_to_return_spec2; eauto. intros. 
+    inv H. inv H0. congruence.
+
+  Case "Ret kernel / user - sym".
+    exploit @c_pop_to_return_spec; eauto.
+    intros [dstk [stk [a [b [p [Hs Hdstk]]]]]]. inv Hs.
+    
+    exploit @c_pop_to_return_spec2; eauto.  move_to_top POP0.
+    exploit @c_pop_to_return_spec2; eauto. intros. 
+    inv H. inv H0. congruence.
+
+  Case "Ret kernel".
+    
+    exploit @c_pop_to_return_spec; eauto.
+    intros [dstk [stk [a [b [p [Hs Hdstk]]]]]]. inv Hs.
+    
+    exploit @c_pop_to_return_spec2; eauto.  move_to_top POP0.
+    exploit @c_pop_to_return_spec2; eauto. intros. 
+    inv H. inv H0. 
+    reflexivity.
+    
+  Case "VRet".
+    exploit @c_pop_to_return_spec; eauto.
+    intros [dstk [stk [a [b [p [Hs Hdstk]]]]]]. inv Hs.
+
+    exploit @c_pop_to_return_spec2; eauto. intros. move_to_top POP0.
+    exploit @c_pop_to_return_spec2; eauto. intros. 
+
+    exploit @c_pop_to_return_spec3; eauto. intros. 
+    generalize POP0 ; clear POP0 ; intros POP0.
+    exploit @c_pop_to_return_spec3; eauto. intros.
+    inv H1.  inv H. inv H0.
+    reflexivity.
+
+  Case "VRet".
+    exploit @c_pop_to_return_spec; eauto.
+    intros [dstk [stk [a [b [p [Hs Hdstk]]]]]]. inv Hs.
+
+    exploit @c_pop_to_return_spec2; eauto. intros. move_to_top POP0.
+    exploit @c_pop_to_return_spec2; eauto. intros. 
+    inv H. inv H0. 
+
+  Case "Ret priv".
     exploit @c_pop_to_return_spec; eauto.
     intros [dstk [stk [a [b [p [Hs Hdstk]]]]]]. inv Hs.
     
@@ -52,21 +130,39 @@ Proof.
     inv H1. inv H2. 
     
     exploit @c_pop_to_return_spec3; eauto. clear H0.
-    exploit @c_pop_to_return_spec3; eauto. intros.
-    inv H1. 
+    exploit @c_pop_to_return_spec3; eauto. 
+    intros.  inv H1.    
     reflexivity.
-    
-  Case "VRet".
+
+  Case "VRet cache hit and miss".
     exploit @c_pop_to_return_spec; eauto.
     intros [dstk [stk [a [b [p [Hs Hdstk]]]]]]. inv Hs.
-
-    exploit @c_pop_to_return_spec2; eauto. intros. move_to_top H13.
+    
+    exploit @c_pop_to_return_spec2; eauto.  move_to_top POP0.
     exploit @c_pop_to_return_spec2; eauto. intros. 
+    inv H. inv H0. 
 
-    exploit @c_pop_to_return_spec3; eauto. intros. 
-    generalize H13 ; clear H13 ; intros H13.
-    exploit @c_pop_to_return_spec3; eauto. intros.
-    inv H1. inv H2.
+  Case "Ret priv".
+    exploit @c_pop_to_return_spec; eauto.
+    intros [dstk [stk [a [b [p [Hs Hdstk]]]]]]. inv Hs.
+    
+    exploit @c_pop_to_return_spec2; eauto.  move_to_top POP0.
+    exploit @c_pop_to_return_spec2; eauto. intros. 
+    inv H. inv H0. 
+    
+    exploit @c_pop_to_return_spec3; eauto. 
+
+  Case "Ret priv true".
+    exploit @c_pop_to_return_spec; eauto.
+    intros [dstk [stk [a [b [p [Hs Hdstk]]]]]]. inv Hs.
+    
+    exploit @c_pop_to_return_spec2; eauto.  move_to_top H13.
+    exploit @c_pop_to_return_spec2; eauto. intros. 
+    inv H1. inv H2. 
+    
+    exploit @c_pop_to_return_spec3; eauto. clear H0.
+    exploit @c_pop_to_return_spec3; eauto. 
+    intros.  inv H1.    
     reflexivity.
 Qed.
 
@@ -88,161 +184,5 @@ Proof.
   inv TAGPC ; inv TAGPC0; congruence.
 Qed.  
 *)
-
-Lemma check_cache_determ: forall opcode labs pcl cs cs' cs'',
-  check_tags opcode labs pcl cs cs' ->
-  check_tags opcode labs pcl cs cs'' ->
-  cs' = cs''.
-Proof.
-  induction 1 ; intros; inv H; auto; try (solve [ intuition]).
-Qed.
- 
-Lemma no_unpriv_step : forall s1, priv s1 = false -> forall s2, ~cstep_p s1 s2.
-Proof.
-  intros. intro S; induction S; simpl in H; try congruence. 
-Qed.
-
-Lemma unpriv_star_step : forall s1, priv s1 = false -> forall s2, star cstep_p s1 s2 -> s1 = s2. 
-Proof.
-  intros.
-  inv H0. 
-   auto.
-   exfalso; eapply no_unpriv_step; eauto.
-Qed.
-
-Lemma no_negpc_step : forall s1, fst (pc s1) < 0 -> forall s2, ~cstep_p s1 s2.
-Proof.
-  intros. intro S; induction S; simpl in H; unfold read_m in *; 
-    case_eq (pcv <? 0); intro C; pose proof (Zlt_cases pcv 0) as Q; try rewrite C in *;
-      congruence.
-Qed.
-
-Lemma negpc_star_step: forall s1, fst (pc s1) < 0 -> forall s2, star cstep_p s1 s2 -> s1 = s2. 
-Proof.
-  intros.
-  inv H0.
-    auto.
-    exfalso; eapply no_negpc_step; eauto.
-Qed.
-
-Lemma runsToEscape_determ: forall cs cs' cs'',
-   runsToEscape cs cs' ->
-   runsToEscape cs cs'' ->
-   cs' = cs''.
-Proof.  (* very tedious. there must be some better lemmas lurking. *)
-  intros. inv H.
-  inv H0. 
-     generalize UPRIV0, STAR0, PRIV0.  clear UPRIV0 STAR0 PRIV0. 
-     induction STAR; intros. 
-       congruence.
-       inv STAR0. 
-         congruence.
-         pose proof (cmach_priv_determ H H0). subst s4.
-         case_eq (priv s2); intros. 
-           eapply IHSTAR; eauto.
-           pose proof (unpriv_star_step H2 STAR). pose proof (unpriv_star_step H2 H1). subst; auto. 
-     generalize FAIL, PRIV1, STAR0, PRIV0.  clear FAIL PRIV1 STAR0 PRIV0.
-     induction STAR; intros.
-       congruence.
-       inv STAR0.
-         exfalso; eapply no_negpc_step; eauto.
-         pose proof (cmach_priv_determ H H0). subst s4.
-         case_eq (priv s2); intros.
-           eapply IHSTAR; eauto. 
-           pose proof (unpriv_star_step H2 STAR). pose proof (unpriv_star_step H2 H1). subst; auto. 
-     congruence.              
-  inv H0. 
-    generalize UPRIV, STAR0, PRIV1, FAIL. clear UPRIV STAR0 PRIV1 FAIL. 
-    induction STAR; intros. 
-      eapply negpc_star_step; eauto.
-      inv STAR0. 
-        congruence.
-         pose proof (cmach_priv_determ H H0). subst s4.
-         case_eq (priv s2); intros. 
-           eapply IHSTAR; eauto. 
-           pose proof (unpriv_star_step H2 STAR). pose proof (unpriv_star_step H2 H1). subst; auto. 
-     generalize FAIL0, PRIV2, STAR0, PRIV1.  clear FAIL0 PRIV2 STAR0 PRIV1.
-     induction STAR; intros.
-       eapply negpc_star_step; eauto. 
-       inv STAR0.
-         exfalso; eapply (no_negpc_step FAIL0); eauto.
-         pose proof (cmach_priv_determ H H0). subst s4.
-         case_eq (priv s2); intros.
-           eapply IHSTAR; eauto. 
-           pose proof (unpriv_star_step H2 STAR). pose proof (unpriv_star_step H2 H1). subst; auto.  
-     congruence.           
-  inv H0. 
-     congruence.
-     congruence.
-     auto.
-Qed.  
-   
-Lemma run_tmu_determ: forall opcode l1 l2 l3 pcl cs cs' cs'',
-  run_tmu opcode l1 l2 l3 pcl cs cs' ->
-  run_tmu opcode l1 l2 l3 pcl cs cs'' ->
-  cs' = cs''.
-Proof.
-  induction 1; intros. inv H2.
-  replace cs'0 with cs' in * by (eapply check_cache_determ ; eauto).
-  eapply runsToEscape_determ; eauto.
-
-Qed.
-
-
-Lemma cache_hit_read_determ: forall c rl1 rpcl1 rl2 rpcl2,
-  cache_hit_read c rl1 rpcl1 -> 
-  cache_hit_read c rl2 rpcl2 ->
-  rl1 = rl2 /\ rpcl1 = rpcl2. 
-Proof.
-  intros. inv H. inv TAG_Res. inv TAG_ResPC. 
-  inv H0. inv TAG_Res. inv TAG_ResPC. 
-  allinv'. allinv'. intuition.
-Qed.
-
-
-Lemma c_pop_to_return_determ : 
-  forall s s1 s2,
-    c_pop_to_return s s1 -> 
-    c_pop_to_return s s2 -> 
-    s1 = s2. 
-Proof. 
-  induction 1; intros.
-  - inv H. reflexivity.
-  - inv H0. eauto.
-Qed.
-
-Lemma cmach_determ: 
-  forall s s' s'', 
-    cstep s s' -> 
-    cstep s s'' -> 
-    s' = s''.
-Proof.
-  induction 1 ; intros;
-  match goal with 
-    | [HH: cstep _ _ |- _ ] => inv HH; try congruence; auto
-  end;
-  repeat (try match goal with
-    | [H1: c_pop_to_return ?S ?S1,
-       H2: c_pop_to_return ?S ?S2 |- _ ] =>
-      let H := fresh in (pose proof (c_pop_to_return_determ H1 H2) as H; eauto; inv H; clear H1 H2)
-    | [H1: run_tmu ?OP ?L1 ?L2 ?L3 ?LPC ?S1 ?S2,
-       H2: run_tmu ?OP ?L1 ?L2 ?L3 ?LPC ?S1 ?S3 |- _] => 
-      let H := fresh in (pose proof (run_tmu_determ H1 H2) as H; eauto; inv H; clear H1 H2)
-    | [H1: cache_hit_read ?C ?RL1 ?RPCL1,
-       H2: cache_hit_read ?C ?RL2 ?RPCL2 |- _] =>
-      let H3 := fresh in let H4 := fresh in 
-         (destruct (cache_hit_read_determ H1 H2) as [H3 H4]; eauto; subst; clear H1 H2)
-  end;
-  try allinv'); 
-  try reflexivity.  
-  (* One remaining case: Call *)
-  Case "call".  
-  try rewrite H13 in *.
-  pose proof (run_tmu_determ H4 H23) as H; eauto; inv H. 
-  destruct (cache_hit_read_determ H5 H24) as [E1 E2]; eauto; subst. 
-  assert (args' = args'0). eapply app_same_length_eq; eauto. intuition. subst.
-  assert (s' = s'0). eapply app_same_length_eq_rest; eauto. intuition.  subst.
-  reflexivity.
-Qed.
 
 End Determinism.
